code/hpke/Hacl.Meta.HPKE.fst
@@ -5,7 +5,11 @@ friend Hacl.Impl.HPKE
 #set-options "--z3rlimit 200 --max_fuel 0 --max_ifuel 0"
 
 %splice[
-  hpke_setupBaseI_higher
+  hpke_setupBaseI_higher;
+  hpke_setupBaseR_higher;
+  hpke_encryptBase_higher
 ] (Meta.Interface.specialize (`Spec.Agile.HPKE.ciphersuite) [
-    `Hacl.Impl.HPKE.setupBaseI
+    `Hacl.Impl.HPKE.setupBaseI;
+    `Hacl.Impl.HPKE.setupBaseR;
+    `Hacl.Impl.HPKE.encryptBase
 ])
